Progress towards vector substitutions (#4)

LeanSubst/Basic.lean
@@ -1,22 +1,78 @@
 
+import Lean.Elab.Term
+import Lean.Elab.SyntheticMVars
+
 namespace LeanSubst
 
 universe u1 u2 u3
 variable {S : Type u1} {T : Type u2} {U : Type u3}
 
+namespace Subst.Syntax
+  open Lean.Elab.Term
+
+  open Lean in
+  def MetaM.promote {α} (x : Meta.MetaM α) : Elab.Term.TermElabM α := x
+
+  def form_list : List Lean.Expr -> TermElabM (Lean.TSyntax `term)
+  | [] => `(List.nil)
+  | .cons x xs => do
+    let xs' <- form_list xs
+    `(List.cons $(<- exprToSyntax x) $xs')
+
+  def form_prod : List Lean.Expr -> TermElabM (Lean.TSyntax `term)
+  | [] => `(PUnit.unit)
+  | .cons x xs => do
+    let xs' <- form_prod xs
+    `(Prod.mk $(<- exprToSyntax x) $xs')
+
+  def get_ty_arg (e : TermElabM Lean.Expr) : TermElabM Lean.Expr := do
+    let e <- e
+    match e with
+    | .app _ ty => pure ty
+    | _ => Lean.Elab.throwUnsupportedSyntax
+end Subst.Syntax
+
+set_option linter.unusedVariables false in
+abbrev Var (T : Type u2) := Nat
+
 structure Ren (T : Type u2) where
   act : Nat -> Nat
 
-class RenMap (S : Type u1) (T : Type u2) where
-  rmap : Ren T -> S -> S
+@[implicit_reducible]
+def RenVec : List (Type u2) -> Type u2
+| [] => PUnit
+| .cons x xs => Ren x × RenVec xs
+
+class RenMap (S : Type u1) (V : List (Type u2)) where
+  rmap : RenVec V -> S -> S
+
+class RenMapAll (V : List (Type u2)) where
+  rmap : ∀ (i : Fin V.length), RenMap V[i] [V[i]]
 
 export RenMap (rmap)
 
-macro:max t:term noWs "⟨" r:term "⟩" : term => `(rmap $r $t)
+macro:max (name := «term_⟨_,⟩») t:term noWs "⟨" r:term ",⟩" : term => `(rmap $r $t)
+syntax:max (name := «term_⟨_,+⟩») term noWs "⟨" term ,+ "⟩" : term
+
+open Lean.Meta in
+open Lean.Elab.Term in
+open Subst.Syntax in
+elab_rules <= expected
+| `($t⟨ $elems,* ⟩) => do
+  let elems <- List.mapM id $ elems.getElems.foldl (λ acc t => elabTermAndSynthesize t none :: acc) []
+  let elems_ty <- List.mapM id $ elems.map inferType |> List.map MetaM.promote |> List.map get_ty_arg
+  let list_ann <- form_list elems_ty.reverse
+  let elems_stx <- form_prod elems.reverse
+  let stx : TermElabM Lean.Syntax := `(@rmap _ $list_ann _ $elems_stx $t)
+  let stx <- stx
+  elabTermAndSynthesize stx expected
 
 @[app_unexpander rmap]
 def unexpand_rmap : Lean.PrettyPrinter.Unexpander
-| `($_ $r $t) => `($t⟨$r⟩)
+| `($_ ($r1, {down := ()}) $t) => `($t⟨$r1⟩)
+| `($_ ($r1, $r2, {down := ()}) $t) => `($t⟨$r1, $r2⟩)
+| `($_ ($r1, $r2, $r3, {down := ()}) $t) => `($t⟨$r1, $r2, $r3⟩)
+| `($_ $r $t) => `($t⟨$r,⟩)
 | _ => throw ()
 
 inductive Action (T : Type u2) where
@@ -29,6 +85,11 @@ export Action (re su)
 structure Subst (T : Type u2) where
   inner : Nat -> Action T
 
+@[implicit_reducible]
+def SubstVec : List (Type u2) -> Type u2
+| [] => PUnit
+| .cons x xs => Subst x × SubstVec xs
+
 class SubstAction (T : Type u1) (A : Type u2) (U : outParam (Type u3)) where
   act (σ : Subst T) : A -> U
 
@@ -37,16 +98,36 @@ def Subst.act [SubstAction S T U] (σ : Subst S) : T -> U := SubstAction.act σ
 instance : SubstAction T Nat (Action T) where
   act := Subst.inner
 
-class SubstMap (S : Type u1) (T : Type u2) where
-  smap : Subst T -> S -> S
+class SubstMap (S : Type u1) (V : List (Type u2)) where
+  smap : SubstVec V -> S -> S
+
+class SubstMapAll (V : List (Type u2)) where
+  smap : ∀ (i : Fin V.length), SubstMap V[i] [V[i]]
 
 export SubstMap (smap)
 
-macro:max t:term noWs "[" σ:term "]" : term => `(smap $σ $t)
+macro:max (name := «term_[_,]») t:term noWs "[" σ:term ",]" : term => `(smap $σ $t)
+syntax:max (name := «term_[_,+]») term noWs "[" term ,+ "]" : term
+
+open Lean.Meta in
+open Lean.Elab.Term in
+open Subst.Syntax in
+elab_rules <= expected
+| `($t[ $elems,* ]) => do
+  let elems <- List.mapM id $ elems.getElems.foldl (λ acc t => elabTermAndSynthesize t none :: acc) []
+  let elems_ty <- List.mapM id $ elems.map inferType |> List.map MetaM.promote |> List.map get_ty_arg
+  let list_ann <- form_list elems_ty.reverse
+  let elems_stx <- form_prod elems.reverse
+  let stx : TermElabM Lean.Syntax := `(@smap _ $list_ann _ $elems_stx $t)
+  let stx <- stx
+  elabTermAndSynthesize stx expected
 
 @[app_unexpander smap]
 def unexpand_smap : Lean.PrettyPrinter.Unexpander
-| `($_ $σ $t) => `($t[$σ])
+| `($_ ($σ1, {down := ()}) $t) => `($t[$σ1])
+| `($_ ($σ1, $σ2, {down := ()}) $t) => `($t[$σ1, $σ2])
+| `($_ ($σ1, $σ2, $σ3, {down := ()}) $t) => `($t[$σ1, $σ2, $σ3])
+| `($_ $σ $t) => `($t[$σ,])
 | _ => throw ()
 
 end LeanSubst
