Examples/VariadicSTLC/Term.lean
@@ -1,0 +1,104 @@
+
+import LeanSubst
+open LeanSubst
+
+namespace VariadicSTLC
+
+inductive Ty where
+| base : Ty
+| arrow : Ty -> Ty
+
+inductive Term where
+| var : Nat -> Term
+| app n : Term -> (Fin n -> Term) -> Term
+| lam n : (Fin n -> Ty) -> Term -> Term
+
+@[coe]
+def Term.from_action : Action Term -> Term
+| re y => var y
+| su t => t
+
+@[simp, grind =]
+theorem Term.from_action_id {n} : from_action (𝐬0.act n) = var n := by
+  simp [from_action]
+
+@[simp, grind =]
+theorem Term.from_action_succ {n} : from_action (𝐬1.act n) = var (n + 1) := by
+  simp [from_action]
+
+@[simp, grind =]
+theorem Term.from_acton_re {n} : from_action (re n) = var n := by simp [from_action]
+
+@[simp, grind =]
+theorem Term.from_action_su {t} : from_action (su t) = t := by simp [from_action]
+
+instance : Coe (Action Term) Term where
+  coe := Term.from_action
+
+@[simp]
+def Term.rmap (r : Ren Term) : Term -> Term
+| var x => var (r.act x)
+| app n t ts => app n (t.rmap r) (λ i => (ts i).rmap r)
+| lam n As t => lam n As (t.rmap $ r.lift n)
+
+instance : RenMap Term [Term] where
+  rmap r := Term.rmap r.1
+
+@[simp, grind =]
+theorem Term.rmap_var {x} {r : Ren Term} : (var x)⟨r⟩ = .var (r.act x) := by
+  simp [RenMap.rmap]
+
+@[simp, grind =]
+theorem Term.rmap_app {n} {t : Term} {ts  : Fin n -> Term} {r : Ren Term}
+  : (app n t ts)⟨r⟩ = app n t⟨r⟩ (λ i => (ts i)⟨r⟩)
+:= by simp [RenMap.rmap]
+
+@[simp, grind =]
+theorem Term.rmap_lam {n As t} {r : Ren Term} : (lam n As t)⟨r⟩ = lam n As t⟨r.lift n⟩ := by
+  simp [RenMap.rmap]
+
+instance : RenMapId Term [Term] where
+  apply_id := by subst_solve_id
+
+instance : RenMapCompose Term [Term] where
+  apply_compose := by sorry
+
+@[simp]
+def Term.smap (σ : Subst Term) : Term -> Term
+| var x => σ.act x
+| app n t ts => app n (t.smap σ) (λ i => (ts i).smap σ)
+| lam n As t => lam n As (t.smap $ σ.lift n)
+
+instance : SubstMap Term [Term] where
+  smap σ := Term.smap σ.1
+
+-- `σ.1.act` might change to `σ[0].act` to prevent things like `σ.2.2.1.act`
+@[simp, grind =]
+theorem Term.smap_var {x} {σ : SubstVec [Term]} : (var x)[σ,] = from_action (σ.1.act x) := by
+  simp [SubstMap.smap]
+
+@[simp, grind =]
+theorem Term.smap_app {n} {t : Term} {ts  : Fin n -> Term} {σ : Subst Term}
+  : (app n t ts)[σ] = app n t[σ] (λ i => (ts i)[σ])
+:= by simp [SubstMap.smap]
+
+@[simp, grind =]
+theorem Term.smap_lam {n As t} {σ : Subst Term} : (lam n As t)[σ] = lam n As t[σ.lift n] := by
+  simp [SubstMap.smap]
+
+instance : SubstMapId Term [Term] where
+  apply_id := by sorry
+
+instance : SubstMapStable Term [Term] where
+  apply_stable := by sorry
+
+instance : SubstMapRenComposeLeft Term [Term] where
+  apply_ren_compose_left := by sorry
+
+instance : SubstMapRenComposeRight Term [Term] where
+  apply_ren_compose_right := by sorry
+
+instance : SubstMapCompose Term [Term] where
+  apply_compose := by sorry
+
+end VariadicSTLC
